src/ndep/SymEvalTests.v
@@ -49,7 +49,11 @@ Module EvaluatorTests (B : Heap) (ST : SepTheoryX.SepTheoryXType B).
     Definition pre_types : list Expr.type := 
       a_type :: b_type :: addr_type :: W_type :: nil.
 
-    Definition funcs : list (signature (wtypes pre_types 2 3)) := nil.
+    (** I need to universally quantify SymEval_word over the functions list
+     **
+     **)
+
+    Definition funcs : functions (wtypes pre_types 2 3) := nil.
 
     Definition sfuncs : list (SEP.ssignature (wtypes pre_types 2 3) (tvType 0) (tvType 1)) :=
       {| SDomain := tvType 2 :: tvType 3 :: nil
@@ -98,7 +102,76 @@ Module EvaluatorTests (B : Heap) (ST : SepTheoryX.SepTheoryXType B).
       admit.
     Defined.
 
-(*
+    Ltac lift_evaluator_w e nt nf :=
+      let r := eval simpl sym_read_word in (sym_read_word e) in
+      let w := eval simpl sym_write_word in (sym_write_word e) in
+      let rc := eval simpl sym_read_word_correct in (sym_read_word_correct e) in
+      let wc := eval simpl sym_write_word_correct in (sym_write_word_correct e) in
+      match type of e with
+        | SymEval_word _ ?stI ?pcI ?ptrI ?wI ?pf _ ?s =>
+          match SE.SEP.lift_ssignatures (s :: nil) nt with
+            | ?s' :: nil =>
+              constr:(@Build_SymEval_word nt stI pcI ptrI wI pf nf s' r w rc wc)
+          end
+      end.
+
+    Check Build_SymEval_word.
+    About DepList.HCons.
+
+    Ltac lift_evaluators_w es nt nf ns :=
+      let rec lift es :=
+        match es with
+          | @DepList.HNil _ (fun n : nat => 
+            match nth_error _ n with
+              | None => Empty_set
+              | Some ss => @SymEval_word _ ?stI ?pcI ?ptrI ?wI ?pf _ _ 
+            end) =>
+            let k := 
+              constr:(@DepList.HNil nat (fun n : nat =>
+                match nth_error ns n with
+                  | None => Empty_set
+                  | Some ss => @SymEval_word nt stI pcI ptrI wI pf nf ss
+                end))
+            in k 
+          | @DepList.HCons _ (fun n : nat => 
+            match nth_error _ n with
+              | None => Empty_set
+              | Some ss => @SymEval_word _ ?stI ?pcI ?ptrI ?wI ?pf _ _ 
+            end) ?f ?ls ?e ?es =>
+          idtac "ok" ;
+            let es := lift es in
+              idtac "here" e ;
+            let e := lift_evaluator_w e nt nf in
+              idtac "got here " ;
+            constr:(@DepList.HCons _ (fun n : nat =>
+                match nth_error ns n with
+                  | None => Empty_set
+                  | Some ss => @SymEval_word nt stI pcI ptrI wI pf nf ss
+                end) f ls e es)
+        end
+      in
+      lift es.
+
+    Goal True.
+      Set Printing Implicit.
+      match goal with
+        | [ |- _ ] => 
+          let z := eval unfold evaluators in evaluators in
+            idtac "foo" z ;
+          let r := lift_evaluators_w z pre_types funcs sfuncs in
+            idtac "here" ;
+            idtac r
+      end.
+
+            constr:(@DepList.HNil nat (fun n : nat => 
+              match nth_error sfuncs n with
+                | None => Empty_set 
+                | Some ss => 
+                  SymEval_word nt addr_not_state
+                  funcs
+                  (pcIndex := 0) (stateIndex := 1) ss
+              end) nil)
+
     Goal forall p1 p2 p3 v1 v2 v3 cs stn m,
       Satisfies cs stn (ST.star (ptsto32 p1 v1) (ST.star (ptsto32 p2 v2) (ptsto32 p3 v3))) m
       -> mem_get_word B.addr B.mem B.footprint_w B.mem_get (IL.implode stn) p1 m = Some v1.
@@ -117,15 +190,22 @@ Module EvaluatorTests (B : Heap) (ST : SepTheoryX.SepTheoryXType B).
           | (?types, ?pcType, ?stateType, ?funcs, ?sfuncs, ?P :: nil) =>
             match SEP.reflect_exprs ltac:(isConst) types funcs (PTR, tt) with
               | (?types, ?funcs, ?PTR :: nil) => 
-                let hyps := constr:(@nil (expr pre_types)) in
+                let hyps := constr:(@nil (expr types)) in
                 let s := eval simpl in (SEP.hash P) in
                 generalize (@symeval_read_word_correct types 1 0 2 3 addr_not_state funcs sfuncs known)
+                  ; pose hyps
 (*
                   hyps PTR (snd s) _ (refl_equal _) CS STN nil nil M I H)
 *)
             end
         end
       end.
+      intros.
+      pose evaluators.
+
+        
+
+      specialize (H0 evaluators).
       (** TODO : the known list needs to be parameterized appropriately... **)
 
       simpl. auto.
